# Proof Export

## Node 1

**Statement:** Let g_1 = (1 6 4 3 7) and g_2 = (1 2 4 5) in S_7 (case n=1, k=m=0). Then [g_1, g_2] := g_1^{-1} g_2^{-1} g_1 g_2 = (1 2 6)(3 4 5).

**Type:** claim

**Inference:** assumption

**Status:** refuted

**Taint:** clean

### Node 1.1

**Statement:** OVERVIEW: We compute the commutator [g_1, g_2] = g_1^{-1} g_2^{-1} g_1 g_2 by tracing all 7 elements of {1,2,3,4,5,6,7} through the composition. Using the convention that (sigma tau)(x) = sigma(tau(x)), we compute [g_1, g_2](x) = g_1^{-1}(g_2^{-1}(g_1(g_2(x)))) for each x. We identify the orbits and express the result in disjoint cycle notation.

**Type:** claim

**Inference:** assumption

**Status:** validated

**Taint:** clean

### Node 1.2

**Statement:** PART 1 - INVERSE VERIFICATION (citing Cycle_Inverse): By Cycle_Inverse, for a cycle (a_1 a_2 ... a_l), the inverse is (a_l ... a_2 a_1), or in standard form starting with the smallest element: (a_1 a_l ... a_2). Applying this: g_1 = (1 6 4 3 7) has inverse (7 3 4 6 1), which in standard form is g_1^{-1} = (1 7 3 4 6). Similarly, g_2 = (1 2 4 5) has inverse (5 4 2 1), which in standard form is g_2^{-1} = (1 5 4 2). These match the given definitions.

**Type:** claim

**Inference:** assumption

**Status:** validated

**Taint:** clean

### Node 1.3

**Statement:** PART 2 - ELEMENT TRACING: We compute [g_1, g_2](x) = g_1^{-1}(g_2^{-1}(g_1(g_2(x)))) for each x in {1,2,3,4,5,6,7}. Action tables: g_1=(1 6 4 3 7): 1->6, 6->4, 4->3, 3->7, 7->1, fixes 2,5. g_2=(1 2 4 5): 1->2, 2->4, 4->5, 5->1, fixes 3,6,7. g_1^{-1}=(1 7 3 4 6): 1->7, 7->3, 3->4, 4->6, 6->1, fixes 2,5. g_2^{-1}=(1 5 4 2): 1->5, 5->4, 4->2, 2->1, fixes 3,6,7.

**Type:** claim

**Inference:** assumption

**Status:** validated

**Taint:** clean

### Node 1.4

**Statement:** TRACE x=1: g_2(1)=2 -> g_1(2)=2 (fixed) -> g_2^{-1}(2)=1 -> g_1^{-1}(1)=7. Therefore 1 maps to 7.

**Type:** claim

**Inference:** assumption

**Status:** validated

**Taint:** clean

### Node 1.5

**Statement:** TRACE x=2: g_2(2)=4 -> g_1(4)=3 -> g_2^{-1}(3)=3 (fixed) -> g_1^{-1}(3)=4. Therefore 2 maps to 4.

**Type:** claim

**Inference:** assumption

**Status:** validated

**Taint:** clean

### Node 1.6

**Statement:** TRACE x=3: g_2(3)=3 (fixed) -> g_1(3)=7 -> g_2^{-1}(7)=7 (fixed) -> g_1^{-1}(7)=3. Therefore 3 maps to 3 (FIXED POINT).

**Type:** claim

**Inference:** assumption

**Status:** validated

**Taint:** clean

### Node 1.7

**Statement:** TRACE x=4: g_2(4)=5 -> g_1(5)=5 (fixed) -> g_2^{-1}(5)=4 -> g_1^{-1}(4)=6. Therefore 4 maps to 6.

**Type:** claim

**Inference:** assumption

**Status:** validated

**Taint:** clean

### Node 1.8

**Statement:** TRACE x=5: g_2(5)=1 -> g_1(1)=6 -> g_2^{-1}(6)=6 (fixed) -> g_1^{-1}(6)=1. Therefore 5 maps to 1.

**Type:** claim

**Inference:** assumption

**Status:** validated

**Taint:** clean

### Node 1.9

**Statement:** TRACE x=6: g_2(6)=6 (fixed) -> g_1(6)=4 -> g_2^{-1}(4)=2 -> g_1^{-1}(2)=2 (fixed). Therefore 6 maps to 2.

**Type:** claim

**Inference:** assumption

**Status:** validated

**Taint:** clean

### Node 1.10

**Statement:** TRACE x=7: g_2(7)=7 (fixed) -> g_1(7)=1 -> g_2^{-1}(1)=5 -> g_1^{-1}(5)=5 (fixed). Therefore 7 maps to 5.

**Type:** claim

**Inference:** assumption

**Status:** validated

**Taint:** clean

#### Node 1.10.1

**Statement:** PART 3 - ORBIT ANALYSIS AND CONCLUSION: From traces 1.4 through 1.10, the complete mapping is: 1->7, 2->4, 3->3 (fixed), 4->6, 5->1, 6->2, 7->5. Identifying orbits: Orbit 1: 1->7->5->1 (3-cycle). Orbit 2: 2->4->6->2 (3-cycle). Orbit 3: 3->3 (fixed point). In cycle notation: [g_1, g_2] = (1 7 5)(2 4 6). IMPORTANT DISCREPANCY: The computed result (1 7 5)(2 4 6) differs from the claimed (1 2 6)(3 4 5). The computation has been verified step-by-step. Either the original claim contains an error, or a different commutator convention was intended.

**Type:** claim

**Inference:** assumption

**Status:** validated

**Taint:** clean

#### Node 1.10.2

**Statement:** ALTERNATIVE COMPUTATION (for reference): Using the alternative commutator definition [g_1, g_2] = g_1 g_2 g_1^{-1} g_2^{-1}, we get: 1->6, 2->1, 3->5, 4->3, 5->4, 6->2, 7->7 (fixed). This gives cycles (1 6 2)(3 5 4), which is the INVERSE of (1 2 6)(3 4 5). This confirms that if the expected answer (1 2 6)(3 4 5) is correct, then the commutator definition should be [g_1, g_2] = g_1 g_2 g_1^{-1} g_2^{-1}, not the one stated in the Commutator definition.

**Type:** claim

**Inference:** assumption

**Status:** validated

**Taint:** clean

